update

Communication_Topology.thy
@@ -56,183 +56,7 @@ abbreviation bind_inr :: "var => bind" ("RIGHT _" [61] 61) where
   "RIGHT x \<equiv> B_Prim (P_Right x)"
   
 value "Map.empty (Var ''x'' \<mapsto> 4)"
-
   
-datatype val = 
-  V_Chan chan ("\<lbrace>_\<rbrace>") |
-  V_Closure prim "var \<rightharpoonup> val" ("\<lbrace>_, _\<rbrace>") |
-  V_Unit ("\<lbrace>\<rbrace>")
-
-
-datatype cont = Cont var exp "var \<rightharpoonup> val" ("\<langle>_,_,_\<rangle>" [0, 0, 0] 70) 
-
-type_synonym state = "exp \<times> (var \<rightharpoonup> val) \<times> cont list"
-  
-type_synonym val_pool = "control_path \<rightharpoonup> val"
-type_synonym state_pool = "control_path \<rightharpoonup> state"
-  
-inductive seq_step :: "state \<Rightarrow> state \<Rightarrow> bool" (infix "\<hookrightarrow>" 55) where 
-  Seq_Result: "
-    (\<rho> x) = Some \<omega> \<Longrightarrow>
-    (RESULT x, \<rho>, \<langle>x_ct, e_ct, \<rho>_ct\<rangle> # \<kappa>) \<hookrightarrow> (e_ct, \<rho>_ct(x_ct \<mapsto> \<omega>), \<kappa>)
-  " |
-  Seq_Let_Unit: "
-    (LET x = \<lparr>\<rparr> in e, \<rho>, \<kappa>) \<hookrightarrow> (e, \<rho>(x \<mapsto> \<lbrace>\<rbrace>), \<kappa>)
-  " |
-  Seq_Let_Prim: "
-    (LET x = B_Prim p in e, \<rho>, \<kappa>) \<hookrightarrow> (e, \<rho>(x \<mapsto> \<lbrace>p, \<rho>\<rbrace>), \<kappa>)
-  " |
-  Seq_Let_Case_Left: "
-    \<lbrakk>(\<rho> x_sum) = Some \<lbrace>P_Left x_ll, \<rho>_l\<rbrace> ; (\<rho>_l x_ll) = Some \<omega>_l \<rbrakk> \<Longrightarrow>
-    (LET x = CASE x_sum LEFT x_l |> e_l RIGHT _ |> _ in e, \<rho>, \<kappa>) \<hookrightarrow> (e_l, \<rho>(x_l \<mapsto> \<omega>_l), \<langle>x, e, \<rho>\<rangle> # \<kappa>)
-  " |
-  Seq_Let_Case_Right: "
-    \<lbrakk>(\<rho> x_sum) = Some \<lbrace>P_Right x_rr, \<rho>_r\<rbrace> ; (\<rho>_r x_rr) = Some \<omega>_r \<rbrakk> \<Longrightarrow>
-    (LET x = CASE x_sum LEFT _ |> _ RIGHT x_r |> e_r in e, \<rho>, \<kappa>) \<hookrightarrow> (e_r, \<rho>(x_r \<mapsto> \<omega>_r), \<langle>x, e, \<rho>\<rangle> # \<kappa>)
-  " |
-  Seq_Fst: "
-    \<lbrakk> (\<rho> x_p) = Some \<lbrace>P_Pair x1 _, \<rho>_p\<rbrace> ; (\<rho>_p x1) = Some \<omega> \<rbrakk> \<Longrightarrow>
-    (LET x = FST x_p in e, \<rho>, \<kappa>) \<hookrightarrow> (e, \<rho>(x \<mapsto> \<omega>), \<kappa>)
-  " |
-  Seq_Snd: "
-    \<lbrakk> (\<rho> x_p) = Some \<lbrace>P_Pair _ x2, \<rho>_p\<rbrace> ; (\<rho>_p x2) = Some \<omega> \<rbrakk> \<Longrightarrow>
-    (LET x = FST x_p in e, \<rho>, \<kappa>) \<hookrightarrow> (e, \<rho>(x \<mapsto> \<omega>), \<kappa>)
-  " |
-  Seq_Let_App: "
-    \<lbrakk>
-      (\<rho> x_f) = Some \<lbrace>P_Abs x_f_abs x_a_abs e_abs, \<rho>_abs\<rbrace> ; 
-      (\<rho> x_a) = Some \<omega>_a 
-    \<rbrakk> \<Longrightarrow>
-    (LET x = APP x_f x_a in e, \<rho>, \<kappa>) \<hookrightarrow> 
-    (e_abs, \<rho>_abs(
-      x_f_abs \<mapsto> \<lbrace>P_Abs x_f_abs x_a_abs e_abs, \<rho>_abs\<rbrace>, 
-      x_a_abs \<mapsto> \<omega>_a
-    ), \<langle>x, e, \<rho>\<rangle> # \<kappa>)
-  "
-  
-inductive seq_steps :: "state \<Rightarrow> state \<Rightarrow> bool" (infix "\<hookrightarrow>*" 55) where
-  Seqs_Refl: "x \<hookrightarrow>* x" |
-  Seqs_Step: "\<lbrakk>x \<hookrightarrow> y ; y \<hookrightarrow>* z\<rbrakk> \<Longrightarrow> x \<hookrightarrow>* z"
-  
-
-abbreviation control_path_append_var :: "control_path => var => control_path" (infixl ";;" 61) where
-  "\<pi>;;x \<equiv> \<pi> @ [Inl x]"
-  
-abbreviation control_path_append_unit :: "control_path  => control_path" ("_;;." [60]61) where
-  "\<pi>;;. \<equiv> \<pi> @ [Inr ()]"
-  
-  
-inductive leaf :: "(control_path \<rightharpoonup> state) \<Rightarrow> control_path \<Rightarrow> bool" where
-  Leaf: "
-    \<lbrakk>
-      (stpool \<pi>) = Some _ ;
-      \<nexists> \<pi>' . (stpool \<pi>') = Some _ \<and> (strict_prefix \<pi> \<pi>')
-    \<rbrakk> \<Longrightarrow>
-    leaf stpool \<pi>
-  "
-
-
-inductive sync_step :: "val_pool \<Rightarrow> val_pool \<Rightarrow> bool" (infix "\<leadsto>" 55) where 
-  Sync_Send_Recv: "
-    \<lbrakk>
-      Some (V_Chan _) = \<rho>_s x_ch_s;
-      \<rho>_r x_ch_r = \<rho>_s x_ch_s ;
-      (\<rho>_s x_m) = Some \<omega>_m
-    \<rbrakk> \<Longrightarrow>
-    vpool(\<pi>_s \<mapsto> \<lbrace>P_Send_Evt x_ch_s x_m, \<rho>_s\<rbrace>, \<pi>_r \<mapsto> \<lbrace>P_Recv_Evt x_ch_r, \<rho>_r\<rbrace>) \<leadsto> 
-    vpool(\<pi>_s \<mapsto> \<lbrace>P_Always_Evt x_a_s, [x_a_s \<mapsto> \<lbrace>\<rbrace>]\<rbrace>, \<pi>_r \<mapsto> \<lbrace>P_Always_Evt x_a_r, [x_a_r \<mapsto> \<omega>_m]\<rbrace>)
-  "
-
-inductive concur_step :: "state_pool \<Rightarrow> state_pool \<Rightarrow> bool" (infix "\<rightarrow>" 55) where 
-  Concur_Lift_Seq: "
-    \<lbrakk> (stpool \<pi>) = Some st; st = (LET x = _ in _, _, _); st \<hookrightarrow> st'\<rbrakk> \<Longrightarrow>
-    stpool \<rightarrow> stpool(\<pi>;;x \<mapsto> st')
-  " |
-  Concur_Lift_Sync: "
-    \<lbrakk>
-      vpool \<leadsto> vpool';
-      (stpool_sync []) = None ;
-      (\<forall> \<pi> x. stpool_sync (\<pi>;;x) = Some _ \<longrightarrow> vpool' \<pi> = Some _ );
-      (\<forall> \<pi> x y. stpool_sync (\<pi>;;x) = Some _ \<longrightarrow> stpool_sync (\<pi>;;y) = Some _ \<longrightarrow> x = y) ;
-      (\<forall> \<pi> .
-        leaf stpool \<pi> \<longrightarrow>
-        (stpool \<pi>) = Some (LET x = SYNC x_evt in e, \<rho>, \<kappa>) \<longrightarrow>
-        (vpool \<pi>) = (\<rho> x_evt) \<longrightarrow>
-        (vpool' \<pi>) = Some \<lbrace>P_Always_Evt x_a, [x_a \<mapsto> \<omega>_a]\<rbrace> \<longrightarrow>
-        stpool_sync (\<pi>;;x) = Some (e, \<rho>(x \<mapsto> \<omega>_a), \<kappa>)
-      )
-    \<rbrakk> \<Longrightarrow>
-    stpool \<rightarrow> stpool ++ stpool_sync
-  " |
-  Concur_Let_Chan: "
-    stpool \<pi> = Some (LET x = CHAN \<lparr>\<rparr> in e, \<rho>, \<kappa>) \<Longrightarrow>
-    stpool \<rightarrow> stpool(
-       \<pi>;;x \<mapsto> (e, \<rho>(x \<mapsto> \<lbrace>Chan (\<pi>;;x)\<rbrace>), \<kappa>)
-    )
-  " |
-  Concur_Let_Spawn: "
-    stpool \<pi> = Some (LET x = SPAWN e_child in e, \<rho>, \<kappa>) \<Longrightarrow>
-    stpool \<rightarrow> stpool(
-      \<pi>;;x \<mapsto> (e, \<rho>(x \<mapsto> \<lbrace>\<rbrace>), \<kappa>), 
-      \<pi>;;. \<mapsto> (e_child, \<rho>, \<kappa>) 
-    )
-  "
-  
-inductive concur_steps :: "state_pool \<Rightarrow> state_pool \<Rightarrow> bool" (infix "\<rightarrow>*" 55) where
-  Concurs_Refl: "x \<rightarrow>* x" |
-  Concurs_Step: "\<lbrakk>x \<rightarrow> y ; y \<rightarrow>* z\<rbrakk> \<Longrightarrow> x \<rightarrow>* z"
-  
-definition send_sites :: "state_pool \<Rightarrow> chan \<Rightarrow> control_path set" where
-  "send_sites stpool ch = {\<pi>. \<exists> x x_evt e \<kappa> \<rho> x_ch x_m \<rho>_evt. 
-    stpool \<pi> = Some (LET x = SYNC x_evt in e, \<rho>, \<kappa>) \<and> 
-    \<rho> x_evt = Some \<lbrace>P_Send_Evt x_ch x_m, \<rho>_evt\<rbrace> \<and> 
-    \<rho>_evt x_ch = Some \<lbrace>ch\<rbrace>
-  }"
-  
-definition recv_sites :: "state_pool \<Rightarrow> chan \<Rightarrow> control_path set" where
-  "recv_sites stpool ch = {\<pi>. \<exists> x x_evt e \<kappa> \<rho> x_ch \<rho>_evt. 
-    stpool \<pi> = Some (LET x = SYNC x_evt in e, \<rho>, \<kappa>) \<and> 
-    \<rho> x_evt = Some \<lbrace>P_Recv_Evt x_ch, \<rho>_evt\<rbrace> \<and> 
-    \<rho>_evt x_ch = Some \<lbrace>ch\<rbrace>
-  }"
-  
-fun channel_exists :: "state_pool \<Rightarrow> chan \<Rightarrow> bool" where
-  "channel_exists stpool (Ch \<pi>) \<longleftrightarrow> (\<exists> x e \<rho> \<kappa>. stpool \<pi> = Some (LET x = CHAN \<lparr>\<rparr> in e, \<rho>, \<kappa>))"
-  
-definition state_pool_possible :: "exp \<Rightarrow> state_pool \<Rightarrow> bool" where
-  "state_pool_possible e stpool \<longleftrightarrow> [[] \<mapsto> (e, Map.empty, [])] \<rightarrow>* stpool"
-  
-definition one_shot :: "exp \<Rightarrow> var \<Rightarrow> bool" where
-  "one_shot e x \<longleftrightarrow> (\<forall> stpool \<pi>. 
-    state_pool_possible e stpool \<longrightarrow>
-    channel_exists stpool (Ch (\<pi>;;x)) \<longrightarrow> (*chan_exists doesn't seem necessary*)
-    card (send_sites stpool (Ch (\<pi>;;x))) \<le> 1
-  )"
-  
-definition single_side :: "(state_pool \<Rightarrow> chan \<Rightarrow> control_path set) \<Rightarrow> exp \<Rightarrow> var \<Rightarrow> bool" where
-  "single_side sites e x \<longleftrightarrow> (\<forall> stpool \<pi> \<pi>_1 \<pi>_2 .
-    state_pool_possible e stpool \<longrightarrow>
-    channel_exists stpool (Ch (\<pi>;;x)) \<longrightarrow>
-    (let site_set = (sites stpool (Ch (\<pi>;;x))) in 
-      \<pi>_1 \<in> site_set \<and> \<pi>_2 \<in> site_set
-    ) \<longrightarrow>
-    (prefix \<pi>_1 \<pi>_2 \<or> prefix \<pi>_2 \<pi>_1) 
-  )"
-  
-definition single_receiver :: "exp \<Rightarrow> var \<Rightarrow> bool" where 
-  "single_receiver = single_side recv_sites"
-  
-definition single_sender :: "exp \<Rightarrow> var \<Rightarrow> bool" where 
-  "single_sender = single_side send_sites"
-  
-definition point_to_point :: "exp \<Rightarrow> var \<Rightarrow> bool" where
-  "point_to_point e x \<longleftrightarrow> single_sender e x \<and> single_receiver e x"
-  
-definition fan_out :: "exp \<Rightarrow> var \<Rightarrow> bool" where
-  "fan_out e x \<longleftrightarrow> single_sender e x \<and> \<not> single_receiver e x "
-  
-definition fan_in :: "exp \<Rightarrow> var \<Rightarrow> bool" where
-  "fan_in e x \<longleftrightarrow> \<not> single_sender e x \<and> single_receiver e x "
 
 
 (* unrestricted grammar*)
@@ -460,7 +284,182 @@ definition normalize :: "u_exp \<Rightarrow> exp" where
   "normalize e = fst (normalize_cont 100 e (\<lambda> i x . (RESULT x, i)))"
 
   
+datatype val = 
+  V_Chan chan ("\<lbrace>_\<rbrace>") |
+  V_Closure prim "var \<rightharpoonup> val" ("\<lbrace>_, _\<rbrace>") |
+  V_Unit ("\<lbrace>\<rbrace>")
+
+
+datatype cont = Cont var exp "var \<rightharpoonup> val" ("\<langle>_,_,_\<rangle>" [0, 0, 0] 70) 
+
+type_synonym state = "exp \<times> (var \<rightharpoonup> val) \<times> cont list"
   
+type_synonym val_pool = "control_path \<rightharpoonup> val"
+type_synonym state_pool = "control_path \<rightharpoonup> state"
+  
+inductive seq_step :: "state \<Rightarrow> state \<Rightarrow> bool" (infix "\<hookrightarrow>" 55) where 
+  Seq_Result: "
+    (\<rho> x) = Some \<omega> \<Longrightarrow>
+    (RESULT x, \<rho>, \<langle>x_ct, e_ct, \<rho>_ct\<rangle> # \<kappa>) \<hookrightarrow> (e_ct, \<rho>_ct(x_ct \<mapsto> \<omega>), \<kappa>)
+  " |
+  Seq_Let_Unit: "
+    (LET x = \<lparr>\<rparr> in e, \<rho>, \<kappa>) \<hookrightarrow> (e, \<rho>(x \<mapsto> \<lbrace>\<rbrace>), \<kappa>)
+  " |
+  Seq_Let_Prim: "
+    (LET x = B_Prim p in e, \<rho>, \<kappa>) \<hookrightarrow> (e, \<rho>(x \<mapsto> \<lbrace>p, \<rho>\<rbrace>), \<kappa>)
+  " |
+  Seq_Let_Case_Left: "
+    \<lbrakk>(\<rho> x_sum) = Some \<lbrace>P_Left x_ll, \<rho>_l\<rbrace> ; (\<rho>_l x_ll) = Some \<omega>_l \<rbrakk> \<Longrightarrow>
+    (LET x = CASE x_sum LEFT x_l |> e_l RIGHT _ |> _ in e, \<rho>, \<kappa>) \<hookrightarrow> (e_l, \<rho>(x_l \<mapsto> \<omega>_l), \<langle>x, e, \<rho>\<rangle> # \<kappa>)
+  " |
+  Seq_Let_Case_Right: "
+    \<lbrakk>(\<rho> x_sum) = Some \<lbrace>P_Right x_rr, \<rho>_r\<rbrace> ; (\<rho>_r x_rr) = Some \<omega>_r \<rbrakk> \<Longrightarrow>
+    (LET x = CASE x_sum LEFT _ |> _ RIGHT x_r |> e_r in e, \<rho>, \<kappa>) \<hookrightarrow> (e_r, \<rho>(x_r \<mapsto> \<omega>_r), \<langle>x, e, \<rho>\<rangle> # \<kappa>)
+  " |
+  Seq_Fst: "
+    \<lbrakk> (\<rho> x_p) = Some \<lbrace>P_Pair x1 _, \<rho>_p\<rbrace> ; (\<rho>_p x1) = Some \<omega> \<rbrakk> \<Longrightarrow>
+    (LET x = FST x_p in e, \<rho>, \<kappa>) \<hookrightarrow> (e, \<rho>(x \<mapsto> \<omega>), \<kappa>)
+  " |
+  Seq_Snd: "
+    \<lbrakk> (\<rho> x_p) = Some \<lbrace>P_Pair _ x2, \<rho>_p\<rbrace> ; (\<rho>_p x2) = Some \<omega> \<rbrakk> \<Longrightarrow>
+    (LET x = FST x_p in e, \<rho>, \<kappa>) \<hookrightarrow> (e, \<rho>(x \<mapsto> \<omega>), \<kappa>)
+  " |
+  Seq_Let_App: "
+    \<lbrakk>
+      (\<rho> x_f) = Some \<lbrace>P_Abs x_f_abs x_a_abs e_abs, \<rho>_abs\<rbrace> ; 
+      (\<rho> x_a) = Some \<omega>_a 
+    \<rbrakk> \<Longrightarrow>
+    (LET x = APP x_f x_a in e, \<rho>, \<kappa>) \<hookrightarrow> 
+    (e_abs, \<rho>_abs(
+      x_f_abs \<mapsto> \<lbrace>P_Abs x_f_abs x_a_abs e_abs, \<rho>_abs\<rbrace>, 
+      x_a_abs \<mapsto> \<omega>_a
+    ), \<langle>x, e, \<rho>\<rangle> # \<kappa>)
+  "
+  
+inductive seq_steps :: "state \<Rightarrow> state \<Rightarrow> bool" (infix "\<hookrightarrow>*" 55) where
+  Seqs_Refl: "x \<hookrightarrow>* x" |
+  Seqs_Step: "\<lbrakk>x \<hookrightarrow> y ; y \<hookrightarrow>* z\<rbrakk> \<Longrightarrow> x \<hookrightarrow>* z"
+  
+
+abbreviation control_path_append_var :: "control_path => var => control_path" (infixl ";;" 61) where
+  "\<pi>;;x \<equiv> \<pi> @ [Inl x]"
+  
+abbreviation control_path_append_unit :: "control_path  => control_path" ("_;;." [60]61) where
+  "\<pi>;;. \<equiv> \<pi> @ [Inr ()]"
+  
+  
+inductive leaf :: "(control_path \<rightharpoonup> state) \<Rightarrow> control_path \<Rightarrow> bool" where
+  Leaf: "
+    \<lbrakk>
+      (stpool \<pi>) = Some _ ;
+      \<nexists> \<pi>' . (stpool \<pi>') = Some _ \<and> (strict_prefix \<pi> \<pi>')
+    \<rbrakk> \<Longrightarrow>
+    leaf stpool \<pi>
+  "
+
+
+inductive sync_step :: "val_pool \<Rightarrow> val_pool \<Rightarrow> bool" (infix "\<leadsto>" 55) where 
+  Sync_Send_Recv: "
+    \<lbrakk>
+      Some (V_Chan _) = \<rho>_s x_ch_s;
+      \<rho>_r x_ch_r = \<rho>_s x_ch_s ;
+      (\<rho>_s x_m) = Some \<omega>_m
+    \<rbrakk> \<Longrightarrow>
+    vpool(\<pi>_s \<mapsto> \<lbrace>P_Send_Evt x_ch_s x_m, \<rho>_s\<rbrace>, \<pi>_r \<mapsto> \<lbrace>P_Recv_Evt x_ch_r, \<rho>_r\<rbrace>) \<leadsto> 
+    vpool(\<pi>_s \<mapsto> \<lbrace>P_Always_Evt x_a_s, [x_a_s \<mapsto> \<lbrace>\<rbrace>]\<rbrace>, \<pi>_r \<mapsto> \<lbrace>P_Always_Evt x_a_r, [x_a_r \<mapsto> \<omega>_m]\<rbrace>)
+  "
+
+inductive concur_step :: "state_pool \<Rightarrow> state_pool \<Rightarrow> bool" (infix "\<rightarrow>" 55) where 
+  Concur_Lift_Seq: "
+    \<lbrakk> (stpool \<pi>) = Some st; st = (LET x = _ in _, _, _); st \<hookrightarrow> st'\<rbrakk> \<Longrightarrow>
+    stpool \<rightarrow> stpool(\<pi>;;x \<mapsto> st')
+  " |
+  Concur_Lift_Sync: "
+    \<lbrakk>
+      vpool \<leadsto> vpool';
+      (stpool_sync []) = None ;
+      (\<forall> \<pi> x. stpool_sync (\<pi>;;x) = Some _ \<longrightarrow> vpool' \<pi> = Some _ );
+      (\<forall> \<pi> x y. stpool_sync (\<pi>;;x) = Some _ \<longrightarrow> stpool_sync (\<pi>;;y) = Some _ \<longrightarrow> x = y) ;
+      (\<forall> \<pi> .
+        leaf stpool \<pi> \<longrightarrow>
+        (stpool \<pi>) = Some (LET x = SYNC x_evt in e, \<rho>, \<kappa>) \<longrightarrow>
+        (vpool \<pi>) = (\<rho> x_evt) \<longrightarrow>
+        (vpool' \<pi>) = Some \<lbrace>P_Always_Evt x_a, [x_a \<mapsto> \<omega>_a]\<rbrace> \<longrightarrow>
+        stpool_sync (\<pi>;;x) = Some (e, \<rho>(x \<mapsto> \<omega>_a), \<kappa>)
+      )
+    \<rbrakk> \<Longrightarrow>
+    stpool \<rightarrow> stpool ++ stpool_sync
+  " |
+  Concur_Let_Chan: "
+    stpool \<pi> = Some (LET x = CHAN \<lparr>\<rparr> in e, \<rho>, \<kappa>) \<Longrightarrow>
+    stpool \<rightarrow> stpool(
+       \<pi>;;x \<mapsto> (e, \<rho>(x \<mapsto> \<lbrace>Chan (\<pi>;;x)\<rbrace>), \<kappa>)
+    )
+  " |
+  Concur_Let_Spawn: "
+    stpool \<pi> = Some (LET x = SPAWN e_child in e, \<rho>, \<kappa>) \<Longrightarrow>
+    stpool \<rightarrow> stpool(
+      \<pi>;;x \<mapsto> (e, \<rho>(x \<mapsto> \<lbrace>\<rbrace>), \<kappa>), 
+      \<pi>;;. \<mapsto> (e_child, \<rho>, \<kappa>) 
+    )
+  "
+  
+inductive concur_steps :: "state_pool \<Rightarrow> state_pool \<Rightarrow> bool" (infix "\<rightarrow>*" 55) where
+  Concurs_Refl: "x \<rightarrow>* x" |
+  Concurs_Step: "\<lbrakk>x \<rightarrow> y ; y \<rightarrow>* z\<rbrakk> \<Longrightarrow> x \<rightarrow>* z"
+  
+definition send_sites :: "state_pool \<Rightarrow> chan \<Rightarrow> control_path set" where
+  "send_sites stpool ch = {\<pi>. \<exists> x x_evt e \<kappa> \<rho> x_ch x_m \<rho>_evt. 
+    stpool \<pi> = Some (LET x = SYNC x_evt in e, \<rho>, \<kappa>) \<and> 
+    \<rho> x_evt = Some \<lbrace>P_Send_Evt x_ch x_m, \<rho>_evt\<rbrace> \<and> 
+    \<rho>_evt x_ch = Some \<lbrace>ch\<rbrace>
+  }"
+  
+definition recv_sites :: "state_pool \<Rightarrow> chan \<Rightarrow> control_path set" where
+  "recv_sites stpool ch = {\<pi>. \<exists> x x_evt e \<kappa> \<rho> x_ch \<rho>_evt. 
+    stpool \<pi> = Some (LET x = SYNC x_evt in e, \<rho>, \<kappa>) \<and> 
+    \<rho> x_evt = Some \<lbrace>P_Recv_Evt x_ch, \<rho>_evt\<rbrace> \<and> 
+    \<rho>_evt x_ch = Some \<lbrace>ch\<rbrace>
+  }"
+  
+fun channel_exists :: "state_pool \<Rightarrow> chan \<Rightarrow> bool" where
+  "channel_exists stpool (Ch \<pi>) \<longleftrightarrow> (\<exists> x e \<rho> \<kappa>. stpool \<pi> = Some (LET x = CHAN \<lparr>\<rparr> in e, \<rho>, \<kappa>))"
+  
+definition state_pool_possible :: "exp \<Rightarrow> state_pool \<Rightarrow> bool" where
+  "state_pool_possible e stpool \<longleftrightarrow> [[] \<mapsto> (e, Map.empty, [])] \<rightarrow>* stpool"
+  
+definition one_shot :: "exp \<Rightarrow> var \<Rightarrow> bool" where
+  "one_shot e x \<longleftrightarrow> (\<forall> stpool \<pi>. 
+    state_pool_possible e stpool \<longrightarrow>
+    (* channel_exists stpool (Ch (\<pi>;;x)) \<longrightarrow> *) (*chan_exists doesn't seem necessary*)
+    card (send_sites stpool (Ch (\<pi>;;x))) \<le> 1
+  )"
+  
+definition single_side :: "(state_pool \<Rightarrow> chan \<Rightarrow> control_path set) \<Rightarrow> exp \<Rightarrow> var \<Rightarrow> bool" where
+  "single_side sites_of e x \<longleftrightarrow> (\<forall> stpool \<pi> \<pi>_1 \<pi>_2 .
+    state_pool_possible e stpool \<longrightarrow>
+    (* channel_exists stpool (Ch (\<pi>;;x)) \<longrightarrow> *)
+    \<pi>_1 \<in> (sites_of stpool (Ch (\<pi>;;x))) \<longrightarrow>
+    \<pi>_2 \<in>(sites_of stpool (Ch (\<pi>;;x))) \<longrightarrow>
+    (prefix \<pi>_1 \<pi>_2 \<or> prefix \<pi>_2 \<pi>_1) 
+  )"  
+  
+definition single_receiver :: "exp \<Rightarrow> var \<Rightarrow> bool" where 
+  "single_receiver = single_side recv_sites"
+  
+definition single_sender :: "exp \<Rightarrow> var \<Rightarrow> bool" where 
+  "single_sender = single_side send_sites"
+  
+definition point_to_point :: "exp \<Rightarrow> var \<Rightarrow> bool" where
+  "point_to_point e x \<longleftrightarrow> single_sender e x \<and> single_receiver e x"
+  
+definition fan_out :: "exp \<Rightarrow> var \<Rightarrow> bool" where
+  "fan_out e x \<longleftrightarrow> single_sender e x \<and> \<not> single_receiver e x "
+  
+definition fan_in :: "exp \<Rightarrow> var \<Rightarrow> bool" where
+  "fan_in e x \<longleftrightarrow> \<not> single_sender e x \<and> single_receiver e x "
+
+    
 abbreviation a where "a \<equiv> Var ''a''"
 abbreviation b where "b \<equiv> Var ''b''"
 abbreviation c where "c \<equiv> Var ''c''"
@@ -489,16 +488,33 @@ definition prog_one where
     LET w = SYNC f in
     RESULT w
   "
-(*
+  
+  
+lemma "\<forall> x . P x \<Longrightarrow> (P 4 \<longrightarrow> Q) \<Longrightarrow> Q"
+  apply (erule mp)
+  apply (drule spec)
+  apply (assumption)
+done
+  
+  
+lemma recv_sites_empty[simp]: "recv_sites [[] \<mapsto> (prog, Map.empty, \<kappa>)] ch = {}"
+by (auto simp add: recv_sites_def)
+    
+  
 theorem prog_one_properties: "
-  single_receiver prog_one a \<and>
-  single_sender prog_one a \<and>
-  single_receiver prog_one c \<and>
-  single_sender prog_one c
+  single_receiver prog_one a
 "
-*) 
+apply (auto simp add: single_receiver_def single_side_def state_pool_possible_def)
+  apply (erule concur_steps.cases)
+   apply (simp)
+   apply (frule_tac P="\<lambda> x . \<pi>_1 \<in> recv_sites x (Ch (\<pi> ;; a)) " in ssubst, assumption)
+   apply (drule_tac P="\<lambda> x . \<pi>_2 \<in> recv_sites x (Ch (\<pi> ;; a))" in ssubst, assumption)
+   apply simp
+  apply simp
+  apply (drule_tac P="\<lambda> x . x \<rightarrow> y" in ssubst, auto)
 
- 
+    
+    
 definition prog_two where 
   "prog_two = 
     .LET a = .CHAN \<lparr>\<rparr> in
