Demos/Auto_Proof_Demo.thy
@@ -1,0 +1,49 @@
+theory Auto_Proof_Demo
+imports Main
+begin
+
+section{* Logic and sets *}
+
+lemma "ALL x. EX y. x=y"
+by auto
+
+lemma "A \<subseteq> B \<inter> C \<Longrightarrow> A \<subseteq> B \<union> C"
+by auto
+
+text{* Note the bounded quantification notation: *}
+
+lemma "\<lbrakk> \<forall>xs \<in> A. \<exists>ys. xs = ys @ ys;  us:A \<rbrakk> \<Longrightarrow> \<exists>n. length us = n+n"
+by fastforce
+
+
+text{*
+ Most simple proofs in FOL and set theory are automatic.
+ Example: if T is total, A is antisymmetric
+ and T is a subset of A, then A is a subset of T.
+*}
+
+lemma AT:
+  "\<lbrakk> \<forall>x y. T x y \<or> T y x;
+     \<forall>x y. A x y \<and> A y x \<longrightarrow> x = y;
+     \<forall>x y. T x y \<longrightarrow> A x y \<rbrakk>
+   \<Longrightarrow> \<forall>x y. A x y \<longrightarrow> T x y"
+by blast
+
+
+section{* Sledgehammer *}
+
+lemma "R^* \<subseteq> (R \<union> S)^*"
+oops
+
+(* Find a suitable P and try sledgehammer: *)
+
+lemma "a # xs = ys @ [a] \<Longrightarrow> P"
+oops
+
+
+section{* Arithmetic *}
+
+lemma "\<forall> (k::nat) > 7. \<exists> i j. k = 3*i + 5*j"
+by arith
+
+end
