Demos/Isar_Induction_Demo.thy
@@ -1,0 +1,191 @@
+theory Isar_Induction_Demo
+imports Main
+begin
+
+section{*Case distinction and induction*}
+
+subsection{*Case distinction*}
+
+text{* Explicit: *}
+
+lemma "length(tl xs) = length xs - 1"
+proof (cases xs)
+  assume "xs = []" thus ?thesis by simp
+next
+  fix y ys assume "xs = y#ys"
+  thus ?thesis by simp
+qed
+
+text{* Implicit: *}
+
+lemma "length(tl xs) = length xs - 1"
+proof (cases xs)
+print_cases
+  case Nil
+thm Nil
+  thus ?thesis by simp
+next
+  case (Cons y ys)
+thm Cons
+  thus ?thesis by simp
+qed
+
+
+subsection{*Structural induction for nat*}
+
+text{* Explicit: *}
+
+lemma "\<Sum>{0..n::nat} = n*(n+1) div 2" (is "?P n")
+proof (induction n)
+  show "?P 0" by simp
+next
+  fix n assume "?P n"
+  thus "?P(Suc n)" by simp
+qed
+
+text{* Implicit: *}
+
+lemma "\<Sum>{0..n::nat} = n*(n+1) div 2"
+proof (induction n)
+print_cases
+  case 0
+  show ?case by simp
+next
+  case (Suc n)
+thm Suc
+  thus ?case by simp
+qed
+
+text{* After the induction or cases step,
+ the PG menu item Isabelle/Show me/cases displays
+ the different cases. *}
+
+text{* Induction with @{text "\<Longrightarrow>"} *}
+
+lemma split_list: "x : set xs \<Longrightarrow> \<exists>ys zs. xs = ys @ x # zs"
+proof (induction xs)
+  case Nil thus ?case by simp
+next
+print_cases
+  case (Cons a xs)
+thm Cons.IH --"Induction hypothesis"
+thm Cons.prems --"Premises of the step case"
+thm Cons
+  from Cons.prems have "x = a \<or> x : set xs" by simp
+  thus ?case
+  proof
+    assume "x = a"
+    hence "a#xs = [] @ x # xs" by simp
+    thus ?thesis by blast
+  next
+    assume "x : set xs"
+    then obtain ys zs where "xs = ys @ x # zs" using Cons.IH by auto
+    hence "a#xs = (a#ys) @ x # zs" by simp
+    thus ?thesis by blast
+  qed
+qed
+
+
+subsection{*Rule induction*}
+
+
+inductive ev :: "nat => bool" where
+ev0:  "ev 0" |
+evSS:  "ev n \<Longrightarrow> ev(Suc(Suc n))"
+
+declare ev.intros [simp]
+
+
+lemma "ev n \<Longrightarrow> \<exists>k. n = 2*k"
+proof (induction rule: ev.induct)
+  case ev0 show ?case by simp
+next
+  case evSS thus ?case by arith
+qed
+
+
+lemma "ev n \<Longrightarrow> \<exists>k. n = 2*k"
+proof (induction rule: ev.induct)
+  case ev0 show ?case by simp
+next
+  case (evSS m)
+thm evSS
+thm evSS.IH
+thm evSS.hyps
+  then obtain k where "m = 2*k" by blast
+  hence "Suc(Suc m) = 2*(k+1)" by simp
+  thus "\<exists>k. Suc(Suc m) = 2*k" by blast
+qed
+
+
+subsection{*Inductive definition of the reflexive transitive closure *}
+
+consts step :: "'a \<Rightarrow> 'a \<Rightarrow> bool" (infix "\<rightarrow>" 55)
+
+inductive steps :: "'a \<Rightarrow> 'a \<Rightarrow> bool" (infix "\<rightarrow>*" 55) where
+refl: "x \<rightarrow>* x" |
+step: "\<lbrakk> x \<rightarrow> y; y \<rightarrow>* z \<rbrakk> \<Longrightarrow> x \<rightarrow>* z"
+
+declare refl[simp, intro]
+
+text{* Explicit and by hand: *}
+
+lemma "x \<rightarrow>* y  \<Longrightarrow>  y \<rightarrow>* z \<Longrightarrow> x \<rightarrow>* z"
+proof(induction rule: steps.induct)
+  fix x assume "x \<rightarrow>* z"
+  thus "x \<rightarrow>* z" . --"by assumption"
+next
+  fix x' x y :: 'a
+  assume "x' \<rightarrow> x" and "x \<rightarrow>* y"
+  assume IH: "y \<rightarrow>* z \<Longrightarrow> x \<rightarrow>* z"
+  assume "y \<rightarrow>* z"
+  show "x' \<rightarrow>* z" by(rule step[OF `x' \<rightarrow> x` IH[OF `y\<rightarrow>*z`]])
+qed
+
+text{* Implicit and automatic: *}
+
+lemma "x \<rightarrow>* y  \<Longrightarrow>  y \<rightarrow>* z \<Longrightarrow> x \<rightarrow>* z"
+proof(induction rule: steps.induct)
+  case refl thus ?case .
+next
+  case (step x' x y)
+  --"x' x y not used in proof text, just for demo"
+thm step
+thm step.IH
+thm step.hyps
+thm step.prems
+  show ?case
+    by (metis step.hyps(1) step.IH step.prems steps.step)
+qed
+
+
+subsection{*Rule inversion*}
+
+
+lemma assumes "ev n" shows "ev(n - 2)"
+proof-
+  from `ev n` show "ev(n - 2)"
+  proof cases
+    case ev0
+thm ev0
+    then show ?thesis by simp
+  next
+    case (evSS k)
+thm evSS
+    then show ?thesis by simp
+  qed
+qed
+
+
+text{* Impossible cases are proved automatically: *}
+
+lemma "\<not> ev(Suc 0)"
+proof
+  assume "ev(Suc 0)"
+  then show False
+  proof cases
+  qed
+qed
+
+
+end
