Demos/Overview_Demo.thy
@@ -1,0 +1,41 @@
+theory Overview_Demo
+imports Main
+begin
+
+(* A simple comment *)
+
+text {* This is also a comment but it generates nice \LaTeX-text! *}
+
+text {* Note that variables and constants (eg True, &) are displayed differently.  *}
+
+term "True"
+term "False"
+term "true"
+term "True & False"
+term "True & false"
+
+value "True & False"
+value "True & P"
+
+(* To display types in jedit: press ctrl (Mac: cmd) and hover over text.
+   To view the definition of a constant: press ctrl (Mac: cmd) and click on the text.
+*)
+
+text {* Warning: "+" and numbers are overloaded: *}
+
+term "n + n = 0"
+term "(n::nat) + n = 0"
+
+(*Try this:
+
+term "True + False"
+
+Terms must be type correct!*)
+
+text{* Type inference: *}
+
+term "f (g x) y"
+term "h (%x. f(g x))"
+term "%x. x + x"
+
+end
