Demos/Single_Step_Demo.thy
@@ -1,0 +1,40 @@
+theory Single_Step_Demo
+imports Main
+begin
+
+text{* "thm" is a command that displays one or more named theorems: *}
+thm conjI impI iffI notI
+
+text{* Instantiation of theorems: "of" *}
+
+text{* Positional: *}
+thm conjI[of "A" "B"]
+thm conjI[of "A"]
+thm conjI[of _ "B"]
+
+text{* By name: *}
+thm conjI[where ?Q = "B"]
+
+text{* Composition of theorems: OF *}
+
+thm refl[of "a"]
+thm conjI[OF refl[of "a"] refl[of "b"]]
+thm conjI[OF refl[of "a"]]
+thm conjI[OF _ refl[of "b"]]
+
+
+text{* A simple backward proof: *}
+lemma "\<lbrakk> A; B \<rbrakk> \<Longrightarrow> A \<and> B"
+apply(rule conjI)
+apply assumption
+apply assumption
+done
+
+text{* Teaching blast new intro rules: *}
+
+thm le_trans
+
+lemma "\<lbrakk> (a::nat) \<le> b; b \<le> c; c \<le> d \<rbrakk> \<Longrightarrow> a \<le> d"
+by(blast intro: le_trans)
+
+end
